Cslib/Foundations/Semantics/LTS/TraceEq.lean
@@ -7,6 +7,7 @@ Authors: Fabrizio Montesi
 module
 
 public import Cslib.Foundations.Semantics.LTS.Basic
+public import Cslib.Foundations.Semantics.LTS.Simulation
 
 @[expose] public section
 
@@ -33,70 +34,71 @@ Definitions and results on trace equivalence for `LTS`s.
 
 namespace Cslib.LTS
 
-universe u v
-
-variable {State : Type u} {Label : Type v} (lts : LTS State Label)
-
 /-- The traces of a state `s` is the set of all lists of labels `μs` such that there is a multi-step
 transition labelled by `μs` originating from `s`. -/
-def traces (s : State) := { μs : List Label | ∃ s', lts.MTr s μs s' }
+def traces (lts : LTS State Label) (s : State) := { μs : List Label | ∃ s', lts.MTr s μs s' }
 
 /-- If there is a multi-step transition from `s` labelled by `μs`, then `μs` is in the traces of
 `s`. -/
-theorem traces_in (s : State) (μs : List Label) (s' : State) (h : lts.MTr s μs s') :
-    μs ∈ lts.traces s := by
-  exists s'
+theorem traces_in {lts : LTS State Label} (h : lts.MTr s μs s') : μs ∈ lts.traces s := by exists s'
 
 /-- Two states are trace equivalent if they have the same set of traces. -/
-def TraceEq (s1 s2 : State) := lts.traces s1 = lts.traces s2
+def TraceEq (lts₁ : LTS State₁ Label) (lts₂ : LTS State₂ Label)
+    (s1 : State₁) (s2 : State₂) :=
+  lts₁.traces s1 = lts₂.traces s2
 
 /--
 Notation for trace equivalence.
 
-Differently from standard pen-and-paper presentations, we require the lts to be mentioned
+Differently from standard pen-and-paper presentations, we require the LTSs to be mentioned
 explicitly.
 -/
-notation s " ~tr[" lts "] " s' => TraceEq lts s s'
+scoped notation s " ~tr[" lts₁ "," lts₂ "] " s' => TraceEq lts₁ lts₂ s s'
 
-/-- Trace equivalence is reflexive. -/
-theorem TraceEq.refl (s : State) : s ~tr[lts] s := by
+/-- Homogeneous trace equivalence compares states on the same LTS. -/
+abbrev HomTraceEq (lts : LTS State Label) := TraceEq lts lts
+
+/-- Notation for homogeneous trace equivalence. -/
+scoped notation s:max " ~tr[" lts "] " s':max => HomTraceEq lts s s'
+
+/-- Homogeneous trace equivalence is reflexive. -/
+theorem HomTraceEq.refl (s : State) : s ~tr[lts] s := by
   simp only [TraceEq]
 
 /-- Trace equivalence is symmetric. -/
-theorem TraceEq.symm (lts : LTS State Label) {s1 s2 : State} (h : s1 ~tr[lts] s2) :
-  s2 ~tr[lts] s1 := by
+theorem TraceEq.symm (h : s1 ~tr[lts₁,lts₂] s2) : s2 ~tr[lts₂,lts₁] s1 := by
   simp only [TraceEq] at h
   simp only [TraceEq]
   rw [h]
 
 /-- Trace equivalence is transitive. -/
-theorem TraceEq.trans {s1 s2 s3 : State} (h1 : s1 ~tr[lts] s2) (h2 : s2 ~tr[lts] s3) :
-  s1 ~tr[lts] s3 := by
+theorem TraceEq.trans (h1 : s1 ~tr[lts₁,lts₂] s2) (h2 : s2 ~tr[lts₂,lts₃] s3) :
+    s1 ~tr[lts₁,lts₃] s3 := by
   simp only [TraceEq] at *
   rw [h1, h2]
 
-/-- Trace equivalence is an equivalence relation. -/
-theorem TraceEq.eqv (lts : LTS State Label) : Equivalence (TraceEq lts) where
-  refl := TraceEq.refl lts
-  symm := TraceEq.symm lts
-  trans := TraceEq.trans lts
+/-- Homogeneous trace equivalence is an equivalence relation. -/
+theorem HomTraceEq.eqv : Equivalence (· ~tr[lts] ·) where
+  refl := HomTraceEq.refl
+  symm := TraceEq.symm
+  trans := TraceEq.trans
 
 /-- `calc` support for simulation equivalence. -/
-instance : Trans (TraceEq lts) (TraceEq lts) (TraceEq lts) where
-  trans := TraceEq.trans lts
+instance : Trans (TraceEq lts₁ lts₂) (TraceEq lts₂ lts₃) (TraceEq lts₁ lts₃) where
+  trans := TraceEq.trans
 
-/-- In a deterministic LTS, trace equivalence is a simulation. -/
-theorem TraceEq.deterministic_sim
-    (lts : LTS State Label) [hdet : lts.Deterministic] (s1 s2 : State) (h : s1 ~tr[lts] s2) :
-    ∀ μ s1', lts.Tr s1 μ s1' → ∃ s2', lts.Tr s2 μ s2' ∧ s1' ~tr[lts] s2' := by
-  intro μ s1' htr1
-  have hmtr1 := MTr.single lts htr1
-  have hin := traces_in lts s1 [μ] s1' hmtr1
+/-- In deterministic LTSs, trace equivalence is a simulation. -/
+theorem TraceEq.deterministic_isSimulation {lts₁ : LTS State₁ Label} {lts₂ : LTS State₂ Label}
+    [hdet₁ : lts₁.Deterministic] [hdet₂ : lts₂.Deterministic] :
+    IsSimulation lts₁ lts₂ (TraceEq lts₁ lts₂) := by
+  intro s1 s2 h μ s1' htr1
+  have hmtr1 := MTr.single lts₁ htr1
+  have hin := traces_in hmtr1
   rw [h] at hin
   obtain ⟨s2', hmtr2⟩ := hin
   exists s2'
   constructor
-  · apply MTr.single_invert lts _ _ _ hmtr2
+  · apply MTr.single_invert lts₂ _ _ _ hmtr2
   · simp only [TraceEq, traces]
     funext μs'
     simp only [eq_iff_iff]
@@ -105,29 +107,29 @@ theorem TraceEq.deterministic_sim
     case mp =>
       intro hmtr1'
       obtain ⟨s1'', hmtr1'⟩ := hmtr1'
-      have hmtr1comp := MTr.comp lts hmtr1 hmtr1'
-      have hin := traces_in lts s1 ([μ] ++ μs') s1'' hmtr1comp
+      have hmtr1comp := MTr.comp lts₁ hmtr1 hmtr1'
+      have hin := traces_in hmtr1comp
       rw [h] at hin
       obtain ⟨s', hmtr2'⟩ := hin
       cases hmtr2'
       case stepL s2'' htr2 hmtr2' =>
         exists s'
-        have htr2' := MTr.single_invert lts _ _ _ hmtr2
-        have hdets2 := hdet.deterministic s2 μ s2' s2'' htr2' htr2
+        have htr2' := MTr.single_invert lts₂ _ _ _ hmtr2
+        have hdets2 := hdet₂.deterministic s2 μ s2' s2'' htr2' htr2
         rw [hdets2]
         exact hmtr2'
     case mpr =>
       intro hmtr2'
       obtain ⟨s2'', hmtr2'⟩ := hmtr2'
-      have hmtr2comp := MTr.comp lts hmtr2 hmtr2'
-      have hin := traces_in lts s2 ([μ] ++ μs') s2'' hmtr2comp
+      have hmtr2comp := MTr.comp lts₂ hmtr2 hmtr2'
+      have hin := traces_in hmtr2comp
       rw [← h] at hin
       obtain ⟨s', hmtr1'⟩ := hin
       cases hmtr1'
       case stepL s1'' htr1 hmtr1' =>
         exists s'
-        have htr1' := MTr.single_invert lts _ _ _ hmtr1
-        have hdets1 := hdet.deterministic s1 μ s1' s1'' htr1' htr1
+        have htr1' := MTr.single_invert lts₁ _ _ _ hmtr1
+        have hdets1 := hdet₁.deterministic s1 μ s1' s1'' htr1' htr1
         rw [hdets1]
         exact hmtr1'
 
